HOLCF-Binary-Join.thy
@@ -1,13 +1,13 @@
-theory "HOLCF-Binary-Meet"
+theory "HOLCF-Binary-Join"
 imports 
-  "Down"
+  "HOLCF"
 begin
 
-subsection {* Binary Meets *}
+subsection {* Binary Joins *}
 
 context pcpo
 begin
-definition meet :: "'a => 'a => 'a" (infix "\<squnion>" 80) where
+definition join :: "'a => 'a => 'a" (infix "\<squnion>" 80) where
   "x \<squnion> y = (if \<exists> z. {x, y} <<| z then lub {x, y} else \<bottom>)"
 
 definition compatible :: "'a \<Rightarrow> 'a \<Rightarrow> bool"
@@ -17,22 +17,22 @@ lemma bot_compatible[simp]:
   "compatible x \<bottom>" "compatible \<bottom> x"
   unfolding compatible_def by (metis insert_commute is_lub_bin minimal)+
 
-lemma meet_idem[simp]: "compatible x y \<Longrightarrow> x \<squnion> (x \<squnion> y) = x \<squnion> y"
+lemma join_idem[simp]: "compatible x y \<Longrightarrow> x \<squnion> (x \<squnion> y) = x \<squnion> y"
 proof-
   assume c1: "compatible x y"
   then obtain z where z:"{x, y} <<| z" unfolding compatible_def by auto
   hence "x \<sqsubseteq> z" by (metis is_lubD1 is_ub_insert)
   hence "{x, z} <<| z" by (metis is_lub_bin)
-  hence "x \<squnion> z = z" unfolding meet_def by (auto intro: lub_eqI)
+  hence "x \<squnion> z = z" unfolding join_def by (auto intro: lub_eqI)
   from z
-  have "x \<squnion> y = z" unfolding meet_def by (auto intro: lub_eqI)
+  have "x \<squnion> y = z" unfolding join_def by (auto intro: lub_eqI)
   hence c2: "compatible x (x \<squnion> y)" unfolding compatible_def using `{x, z} <<| z` by auto
   
   show ?thesis using `x \<squnion> y = z` `x \<squnion> z = z` by auto
 qed
 
-lemma meet_self[simp]: "x \<squnion> x = x"
-  unfolding meet_def
+lemma join_self[simp]: "x \<squnion> x = x"
+  unfolding join_def
   apply auto
   apply (metis is_lub_singleton)
   done
@@ -50,7 +50,7 @@ proof-
   thus ?thesis unfolding compatible_def by (metis)
 qed
 
-lemma is_meetI:
+lemma is_joinI:
   assumes "x \<sqsubseteq> z"
   assumes "y \<sqsubseteq> z"
   assumes "\<And> a. \<lbrakk> x \<sqsubseteq> a ; y \<sqsubseteq> a \<rbrakk> \<Longrightarrow> z \<sqsubseteq> a"
@@ -59,15 +59,15 @@ proof-
   from assms
   have "{x,y} <<| z"
     by (auto intro: is_lubI)
-  thus ?thesis unfolding meet_def by (metis lub_eqI)
+  thus ?thesis unfolding join_def by (metis lub_eqI)
 qed
 
-lemma lub_is_meet:
+lemma lub_is_join:
   "{x, y} <<| z \<Longrightarrow> x \<squnion> y = z"
-unfolding meet_def by (metis lub_eqI)
+unfolding join_def by (metis lub_eqI)
 
 
-lemma meet_mono:
+lemma join_mono:
   assumes "compatible a b"
   and "compatible c d"
   and "a \<sqsubseteq> c"
@@ -78,21 +78,21 @@ proof-
   with assms have "a \<sqsubseteq> y" "b \<sqsubseteq> y" by (metis below.r_trans is_lubD1 is_ub_insert)+
   with `{a, b} <<| x` have "x \<sqsubseteq> y" by (metis is_lub_below_iff is_lub_singleton is_ub_insert)
   moreover
-  from `{a, b} <<| x` `{c, d} <<| y` have "a \<squnion> b = x" "c \<squnion> d = y" by (metis lub_is_meet)+
+  from `{a, b} <<| x` `{c, d} <<| y` have "a \<squnion> b = x" "c \<squnion> d = y" by (metis lub_is_join)+
   ultimately
   show ?thesis by simp
 qed
 
 lemma
   assumes "compatible x y"
-  shows meet_above1: "x \<sqsubseteq> x \<squnion> y" and meet_above2: "y \<sqsubseteq> x \<squnion> y"
+  shows join_above1: "x \<sqsubseteq> x \<squnion> y" and join_above2: "y \<sqsubseteq> x \<squnion> y"
 proof-
   from assms obtain z where "{x,y} <<| z" unfolding compatible_def by auto
-  hence  "x \<squnion> y = z" and "x \<sqsubseteq> z" and "y \<sqsubseteq> z" apply (auto intro: lub_is_meet) by (metis is_lubD1 is_ub_insert)+
+  hence  "x \<squnion> y = z" and "x \<sqsubseteq> z" and "y \<sqsubseteq> z" apply (auto intro: lub_is_join) by (metis is_lubD1 is_ub_insert)+
   thus "x \<sqsubseteq> x \<squnion> y" and "y \<sqsubseteq> x \<squnion> y" by simp_all
 qed
 
-lemma meet_below:
+lemma join_below:
   assumes "compatible x y"
   and "x \<sqsubseteq> a" and "y \<sqsubseteq> a"
   shows "x \<squnion> y \<sqsubseteq> a"
@@ -100,7 +100,7 @@ proof-
   from assms obtain z where z: "{x,y} <<| z" unfolding compatible_def by auto
   with assms have "z \<sqsubseteq> a" by (metis is_lub_below_iff is_ub_empty is_ub_insert)
   moreover
-  from z have "x \<squnion> y = z" by (rule lub_is_meet) 
+  from z have "x \<squnion> y = z" by (rule lub_is_join) 
   ultimately show ?thesis by simp
 qed
 
@@ -114,17 +114,17 @@ proof(rule admI)
   proof(rule compatibleI)
     have c2: "chain (\<lambda>i. x \<squnion> Y i)"
       apply (rule chainI)
-      apply (rule meet_mono[OF a a below_refl chainE[OF `chain Y`]])
+      apply (rule join_mono[OF a a below_refl chainE[OF `chain Y`]])
       done
     show "x \<sqsubseteq> (\<Squnion> i. x \<squnion> Y i)"
-      by (auto intro: admD[OF _ c2] meet_above1[OF a])
+      by (auto intro: admD[OF _ c2] join_above1[OF a])
     show "(\<Squnion> i. Y i) \<sqsubseteq> (\<Squnion> i. x \<squnion> Y i)"
-      by (auto intro: admD[OF _ c] below_lub[OF c2 meet_above2[OF a]])
+      by (auto intro: admD[OF _ c] below_lub[OF c2 join_above2[OF a]])
     fix a
     assume "x \<sqsubseteq> a" and "(\<Squnion> i. Y i) \<sqsubseteq> a"
     show "(\<Squnion> i. x \<squnion> Y i) \<sqsubseteq> a"
       apply (rule lub_below[OF c2])
-      apply (rule meet_below[OF a `x \<sqsubseteq> a`])
+      apply (rule join_below[OF a `x \<sqsubseteq> a`])
       apply (rule below_trans[OF is_ub_thelub[OF c] `(\<Squnion> i. Y i) \<sqsubseteq> a`])
       done
   qed
