Denotational.thy
@@ -8,7 +8,7 @@ where
   "atom x \<sharp> \<rho> ==> \<lbrakk> Lam [x]. e \<rbrakk>\<^bsub>\<rho>\<^esub> = Fn \<cdot> (\<Lambda> v. (\<lbrakk> e \<rbrakk>\<^bsub>\<rho>(x f\<mapsto> v)\<^esub>))"
 | "\<lbrakk> App e x \<rbrakk>\<^bsub>\<rho>\<^esub> = \<lbrakk> e \<rbrakk>\<^bsub>\<rho>\<^esub> \<down>Fn \<lbrakk> Var x \<rbrakk>\<^bsub>\<rho>\<^esub> "
 | "\<lbrakk> Var x \<rbrakk>\<^bsub>\<rho>\<^esub> = the (lookup \<rho> x)"
-| "set (bn as) \<sharp>* \<rho> \<Longrightarrow>\<lbrakk>Let as body\<rbrakk>\<^bsub>\<rho>\<^esub> = \<lbrakk>body\<rbrakk>\<^bsub>heapExtendMeet \<rho> (asToHeap as) ESem\<^esub>"
+| "set (bn as) \<sharp>* \<rho> \<Longrightarrow>\<lbrakk>Let as body\<rbrakk>\<^bsub>\<rho>\<^esub> = \<lbrakk>body\<rbrakk>\<^bsub>heapExtendJoin \<rho> (asToHeap as) ESem\<^esub>"
 proof-
 case goal1 thus ?case
   unfolding eqvt_def ESem_graph_def
@@ -55,17 +55,17 @@ next
 
 case (goal13 as \<rho> body as' \<rho>' body')
   assume eqvt1: "\<And> e x. e \<in> snd ` set (asToHeap as) \<Longrightarrow> eqvt_at ESem_sumC (e, x)"
-    and eqvt2:"eqvt_at ESem_sumC (body, heapExtendMeet \<rho> (asToHeap as) (\<lambda>x0 x1. ESem_sumC (x0, x1)))"
+    and eqvt2:"eqvt_at ESem_sumC (body, heapExtendJoin \<rho> (asToHeap as) (\<lambda>x0 x1. ESem_sumC (x0, x1)))"
     and eqvt3:"\<And>e x. e \<in> snd ` set (asToHeap as') \<Longrightarrow> eqvt_at ESem_sumC (e, x)"
-    and eqvt4:"eqvt_at ESem_sumC (body', heapExtendMeet \<rho>' (asToHeap as') (\<lambda>x0 x1. ESem_sumC (x0, x1)))"
+    and eqvt4:"eqvt_at ESem_sumC (body', heapExtendJoin \<rho>' (asToHeap as') (\<lambda>x0 x1. ESem_sumC (x0, x1)))"
 
   assume fresh1: "set (bn as) \<sharp>* \<rho>" and fresh2: "set (bn as') \<sharp>* \<rho>'"
   assume "(Terms.Let as body, \<rho>) =  (Terms.Let as' body', \<rho>')"
   hence tmp: "[bn as]lst. (body, as) = [bn as']lst. (body', as')" and rho:"\<rho>' = \<rho>" by auto
 
-  have "ESem_sumC (body, heapExtendMeet \<rho> (asToHeap as) (\<lambda>x0 x1. ESem_sumC (x0, x1))) =
-        ESem_sumC (body', heapExtendMeet \<rho> (asToHeap as') (\<lambda>x0 x1. ESem_sumC (x0, x1)))"
-    apply (rule Abs_lst_fcb[of bn _ _ _ _ "(\<lambda> as (body, as'). ESem_sumC (body, heapExtendMeet \<rho> (asToHeap as) (\<lambda>x0 x1. ESem_sumC (x0, x1))))" , OF tmp, simplified])
+  have "ESem_sumC (body, heapExtendJoin \<rho> (asToHeap as) (\<lambda>x0 x1. ESem_sumC (x0, x1))) =
+        ESem_sumC (body', heapExtendJoin \<rho> (asToHeap as') (\<lambda>x0 x1. ESem_sumC (x0, x1)))"
+    apply (rule Abs_lst_fcb[of bn _ _ _ _ "(\<lambda> as (body, as'). ESem_sumC (body, heapExtendJoin \<rho> (asToHeap as) (\<lambda>x0 x1. ESem_sumC (x0, x1))))" , OF tmp, simplified])
     apply (rule pure_fresh)+
     apply (erule conjE)
     using fresh2[unfolded rho]
@@ -84,11 +84,11 @@ case (goal13 as \<rho> body as' \<rho>' body')
         apply (rule perm_supp_eq)
         apply (auto intro: perm_supp_eq simp add: fresh_star_def)
         done            
-      thus "\<pi> \<bullet> ESem_sumC (body, heapExtendMeet \<rho> (asToHeap as) (\<lambda>x0 x1. ESem_sumC (x0, x1))) =
-             ESem_sumC (body', heapExtendMeet \<rho> (asToHeap as') (\<lambda>x0 x1. ESem_sumC (x0, x1)))"
+      thus "\<pi> \<bullet> ESem_sumC (body, heapExtendJoin \<rho> (asToHeap as) (\<lambda>x0 x1. ESem_sumC (x0, x1))) =
+             ESem_sumC (body', heapExtendJoin \<rho> (asToHeap as') (\<lambda>x0 x1. ESem_sumC (x0, x1)))"
          using as body         
-         apply (simp add: eqvt2[unfolded eqvt_at_def, simplified, rule_format]   asToHeap.eqvt heapExtendMeet_eqvt)
-         apply (subst heapExtendMeet_cong)
+         apply (simp add: eqvt2[unfolded eqvt_at_def, simplified, rule_format]   asToHeap.eqvt heapExtendJoin_eqvt)
+         apply (subst heapExtendJoin_cong)
          prefer 4
          apply (rule refl)+
          apply (simp add: permute_fun_def)
@@ -103,8 +103,8 @@ case (goal13 as \<rho> body as' \<rho>' body')
          apply simp
          done
     qed
-  thus "ESem_sumC (body, heapExtendMeet \<rho> (asToHeap as) (\<lambda>x0 x1. ESem_sumC (x0, x1))) =
-      ESem_sumC (body', heapExtendMeet \<rho>' (asToHeap as') (\<lambda>x0 x1. ESem_sumC (x0, x1)))" using `\<rho>' = \<rho>`  by simp
+  thus "ESem_sumC (body, heapExtendJoin \<rho> (asToHeap as) (\<lambda>x0 x1. ESem_sumC (x0, x1))) =
+      ESem_sumC (body', heapExtendJoin \<rho>' (asToHeap as') (\<lambda>x0 x1. ESem_sumC (x0, x1)))" using `\<rho>' = \<rho>`  by simp
 qed auto
 
 lemma  True and [simp]:"(a, b) \<in> set (asToHeap as) \<Longrightarrow> size b < Suc (size as + size body)"
